Make PositiveAccounts theorems strictly greater than 0

isabelle/PositiveAccounts.thy
@@ -2,156 +2,163 @@ theory PositiveAccounts
 imports Semantics ValidState
 begin
 
+fun positiveMoneyInAccountOrNoAccount :: "AccountId \<Rightarrow> ((AccountId \<times> Money) list) \<Rightarrow> bool" where
+"positiveMoneyInAccountOrNoAccount accId mlist =
+  (case MList.lookup accId mlist of
+     None \<Rightarrow> True
+   | Some x \<Rightarrow> x > 0)"
+
 lemma addMoneyToAccountPositve_match :
- "\<forall>x. 0 \<le> moneyInAccount x accs \<Longrightarrow>
+ "\<forall>x. positiveMoneyInAccountOrNoAccount x accs \<Longrightarrow>
     money > 0 \<Longrightarrow>
     newBalance > 0 \<Longrightarrow>
-    0 \<le> moneyInAccount y (MList.insert y newBalance accs)"
+    positiveMoneyInAccountOrNoAccount y (MList.insert y newBalance accs)"
   apply simp
   by (simp add: MList.insert_lookup_Some)
 
 lemma addMoneyToAccountPositive_noMatch :
- "\<forall>x. 0 \<le> moneyInAccount x accs \<Longrightarrow>
+ "\<forall>x. positiveMoneyInAccountOrNoAccount x accs \<Longrightarrow>
     money > 0 \<Longrightarrow>
     accId \<noteq> y \<Longrightarrow>
     newBalance > 0 \<Longrightarrow>
-    0 \<le> moneyInAccount y (MList.insert accId newBalance accs)"
+    positiveMoneyInAccountOrNoAccount y (MList.insert accId newBalance accs)"
   apply simp
   by (simp add: insert_lookup_different)
 
-lemma updateMoneyInAccount_geZero :
+lemma updateMoneyInAccount_gtZero :
  "0 < newBalance \<Longrightarrow>
-  \<forall>x. 0 \<le> moneyInAccount x accs \<Longrightarrow>
-  0 \<le> moneyInAccount y (updateMoneyInAccount accId newBalance accs)"
+  \<forall>x. positiveMoneyInAccountOrNoAccount x accs \<Longrightarrow>
+  positiveMoneyInAccountOrNoAccount y (updateMoneyInAccount accId newBalance accs)"
   by (metis addMoneyToAccountPositive_noMatch addMoneyToAccountPositve_match not_less updateMoneyInAccount.simps)
 
 lemma addMoneyToAccountPositive :
-  "0 \<le> money \<Longrightarrow> (\<forall>x. moneyInAccount x accs \<ge> 0)
-  \<Longrightarrow> moneyInAccount y (addMoneyToAccount accId money accs) \<ge> 0"
+  "0 \<le> money \<Longrightarrow> (\<forall>x. positiveMoneyInAccountOrNoAccount x accs)
+  \<Longrightarrow> positiveMoneyInAccountOrNoAccount y (addMoneyToAccount accId money accs)"
   apply (simp only:"addMoneyToAccount.simps")
   apply (cases "money \<le> 0")
   apply simp
-  apply (simp del:moneyInAccount.simps)
-  apply (cases "accId = y")
-  apply (smt updateMoneyInAccount.simps updateMoneyInAccount_geZero)
-  by (smt updateMoneyInAccount.simps updateMoneyInAccount_geZero)
+  apply (cases "lookup accId accs")
+  apply simp
+  apply (metis (full_types) MList.insert_lookup_Some insert_lookup_different not_less option.simps(5))
+  apply simp
+  by (smt MList.insert_lookup_Some insert_lookup_different option.simps(5))
 
-lemma giveMoney_geZero :
-    "\<forall>x. 0 \<le> moneyInAccount x accs \<Longrightarrow>
+lemma giveMoney_gtZero :
+    "\<forall>x. positiveMoneyInAccountOrNoAccount x accs \<Longrightarrow>
        (eff, newAccs) = giveMoney payee money accs \<Longrightarrow>
-       0 \<le> moneyInAccount y newAccs"
+       positiveMoneyInAccountOrNoAccount y newAccs"
   by (metis addMoneyToAccount.simps addMoneyToAccountPositive giveMoney.elims linear snd_conv)
 
-lemma moneyInAccount_valid_zero : "valid_map ((accId, money) # rest) \<Longrightarrow> moneyInAccount accId rest = 0"
-  apply (simp only:moneyInAccount.simps findWithDefault.simps)
+lemma positiveMoneyInAccountOrNoAccount_valid_zero : "valid_map ((accId, money) # rest) \<Longrightarrow> positiveMoneyInAccountOrNoAccount accId rest"
+  apply (simp only:positiveMoneyInAccountOrNoAccount.simps findWithDefault.simps)
   by (simp add: MList.delete_lookup_None_aux)
 
-lemma moneyInAccount_sublist_geZero_different :
+lemma positiveMoneyInAccountOrNoAccount_sublist_gtZero_different :
   "valid_map ((accId, money) # rest) \<Longrightarrow>
-   0 < money \<Longrightarrow> 0 \<le> moneyInAccount y ((accId, money) # rest) \<Longrightarrow>
-   accId \<noteq> y \<Longrightarrow> 0 \<le> moneyInAccount y rest"
-  apply (simp only:moneyInAccount.simps findWithDefault.simps)
+   0 < money \<Longrightarrow> positiveMoneyInAccountOrNoAccount y ((accId, money) # rest) \<Longrightarrow>
+   accId \<noteq> y \<Longrightarrow> positiveMoneyInAccountOrNoAccount y rest"
+  apply (simp only:positiveMoneyInAccountOrNoAccount.simps findWithDefault.simps)
   by (metis MList.delete.simps(2) MList.different_delete_lookup)
 
-lemma moneyInAccount_sublist_geZero :
+lemma positiveMoneyInAccountOrNoAccount_sublist_gtZero :
     "valid_map ((accId, money) # rest) \<Longrightarrow>
      money > 0 \<Longrightarrow>
-    (\<forall>x. 0 \<le> moneyInAccount x ((accId, money) # rest)) \<Longrightarrow> 0 \<le> moneyInAccount y rest"
+    (\<forall>x. positiveMoneyInAccountOrNoAccount x ((accId, money) # rest)) \<Longrightarrow> positiveMoneyInAccountOrNoAccount y rest"
   apply (cases "accId = y")
-  using moneyInAccount_valid_zero apply auto[1]
-  using moneyInAccount_sublist_geZero_different by blast
+  using positiveMoneyInAccountOrNoAccount_valid_zero apply auto[1]
+  using positiveMoneyInAccountOrNoAccount_sublist_gtZero_different by blast
 
-lemma moneyInAccount_geZero_preservation :
+lemma positiveMoneyInAccountOrNoAccount_gtZero_preservation :
   "valid_map ((accId, money) # rest) \<Longrightarrow>
-   (\<forall>x. 0 \<le> moneyInAccount x ((accId, money) # rest)) \<Longrightarrow> 0 \<le> moneyInAccount y rest"
-  apply (simp only:moneyInAccount.simps findWithDefault.simps)
-  by (metis MList.delete.simps(2) MList.delete_lookup_None_aux MList.delete_valid_aux MList.insert_in_middle lookup.simps(2) not_less_iff_gr_or_eq option.simps(4) order_refl)
+   (\<forall>x. positiveMoneyInAccountOrNoAccount x ((accId, money) # rest)) \<Longrightarrow> positiveMoneyInAccountOrNoAccount y rest"
+  apply (simp only:positiveMoneyInAccountOrNoAccount.simps findWithDefault.simps)
+  by (metis lookup.simps(2) option.simps(5) positiveMoneyInAccountOrNoAccount.simps positiveMoneyInAccountOrNoAccount_sublist_gtZero)
 
-lemma reduceOne_geZero_aux :
+lemma reduceOne_gtZero_aux :
   "valid_map ((accId, money) # rest) \<Longrightarrow>
-   (money \<le> 0 \<Longrightarrow> \<forall>x. 0 \<le> moneyInAccount x rest \<Longrightarrow> refundOne rest = Some (paym, newAccs) \<Longrightarrow> 0 \<le> moneyInAccount y newAccs) \<Longrightarrow>
-   \<forall>x. 0 \<le> moneyInAccount x ((accId, money) # rest) \<Longrightarrow> refundOne ((accId, money) # rest) = Some (paym, newAccs) \<Longrightarrow> 0 \<le> moneyInAccount y newAccs"
+   (money \<le> 0 \<Longrightarrow> \<forall>x. positiveMoneyInAccountOrNoAccount x rest \<Longrightarrow> refundOne rest = Some (paym, newAccs) \<Longrightarrow> positiveMoneyInAccountOrNoAccount y newAccs) \<Longrightarrow>
+   \<forall>x. positiveMoneyInAccountOrNoAccount x ((accId, money) # rest) \<Longrightarrow> refundOne ((accId, money) # rest) = Some (paym, newAccs) \<Longrightarrow> positiveMoneyInAccountOrNoAccount y newAccs"
   apply (cases "money > 0")
   apply (simp only:refundOne.simps)
-  using moneyInAccount_sublist_geZero apply auto[1]
+  using positiveMoneyInAccountOrNoAccount_sublist_gtZero apply auto[1]
   apply (simp only:refundOne.simps if_False)
-  using moneyInAccount_geZero_preservation not_less by blast
+  using positiveMoneyInAccountOrNoAccount_gtZero_preservation not_less by blast
 
-lemma reduceOne_geZero :
+lemma reduceOne_gtZero :
   "valid_map accs \<Longrightarrow>
-   \<forall>x. 0 \<le> moneyInAccount x accs \<Longrightarrow>
+   \<forall>x. positiveMoneyInAccountOrNoAccount x accs \<Longrightarrow>
    refundOne accs = Some (paym, newAccs) \<Longrightarrow>
-   0 \<le> moneyInAccount y newAccs"
+   positiveMoneyInAccountOrNoAccount y newAccs"
   apply (induction accs rule:"refundOne.induct")
-  apply (meson MList.sublist_valid not_le reduceOne_geZero_aux)
+  apply (meson MList.sublist_valid not_le reduceOne_gtZero_aux)
   by auto
 
-lemma reduceContractStep_geZero_Refund_aux :
+lemma reduceContractStep_gtZero_Refund_aux :
   "valid_state state \<Longrightarrow>
-   \<forall>x. 0 \<le> moneyInAccount x (accounts state) \<Longrightarrow>
+   \<forall>x. positiveMoneyInAccountOrNoAccount x (accounts state) \<Longrightarrow>
    refundOne (accounts state) = Some ((party, money), newAccount) \<Longrightarrow>
    wa = ReduceNoWarning \<Longrightarrow>
    eff = ReduceWithPayment (Payment party money) \<Longrightarrow>
-   0 \<le> moneyInAccount y newAccount"
-  using reduceOne_geZero valid_state.elims(2) by blast
+   positiveMoneyInAccountOrNoAccount y newAccount"
+  using reduceOne_gtZero valid_state.elims(2) by blast
 
-lemma reduceContractStep_geZero_Refund :
+lemma reduceContractStep_gtZero_Refund :
   "valid_state state \<Longrightarrow>
-   \<forall>x. 0 \<le> moneyInAccount x (accounts state) \<Longrightarrow>
+   \<forall>x. positiveMoneyInAccountOrNoAccount x (accounts state) \<Longrightarrow>
    refundOne (accounts state) = Some ((party, money), newAccount) \<Longrightarrow>
    Reduced ReduceNoWarning (ReduceWithPayment (Payment party money)) (state\<lparr>accounts := newAccount\<rparr>) Close =
       Reduced wa eff newState newCont \<Longrightarrow>
-   0 \<le> moneyInAccount y (accounts newState)"
-  using reduceContractStep_geZero_Refund_aux by auto
+   positiveMoneyInAccountOrNoAccount y (accounts newState)"
+  using reduceContractStep_gtZero_Refund_aux by auto
 
-lemma MList_delete_preserves_geZero : "valid_map accs \<Longrightarrow> \<forall>x. 0 \<le> moneyInAccount x accs \<Longrightarrow>
-                                       0 \<le> moneyInAccount y (MList.delete accId accs)"
-  by (metis MList.delete_lookup_None MList.delete_lookup_None_aux MList.delete_valid MList.different_delete_lookup eq_iff findWithDefault.simps moneyInAccount.simps moneyInAccount_valid_zero refundOne.elims)
+lemma MList_delete_preserves_gtZero : "valid_map accs \<Longrightarrow> \<forall>x. positiveMoneyInAccountOrNoAccount x accs \<Longrightarrow>
+                                       positiveMoneyInAccountOrNoAccount y (MList.delete accId accs)"
+  by (metis (full_types) MList.delete_lookup_None MList.different_delete_lookup option.simps(4) positiveMoneyInAccountOrNoAccount.simps)
 
-lemma reduceContractStep_geZero_Pay_aux :
+lemma reduceContractStep_gtZero_Pay_aux :
   "valid_state state \<Longrightarrow>
-   \<forall>x. 0 \<le> moneyInAccount x (accounts state) \<Longrightarrow>
-   0 \<le> moneyInAccount x (updateMoneyInAccount accId amount (accounts state))"
-  using MList_delete_preserves_geZero updateMoneyInAccount_geZero by auto
+   \<forall>x. positiveMoneyInAccountOrNoAccount x (accounts state) \<Longrightarrow>
+   positiveMoneyInAccountOrNoAccount x (updateMoneyInAccount accId amount (accounts state))"
+  using MList_delete_preserves_gtZero updateMoneyInAccount_gtZero by auto
 
-lemma reduceContractStep_geZero_Pay :
+lemma reduceContractStep_gtZero_Pay :
   "valid_state state \<Longrightarrow>
-   \<forall>x. 0 \<le> moneyInAccount x (accounts state) \<Longrightarrow>
+   \<forall>x. positiveMoneyInAccountOrNoAccount x (accounts state) \<Longrightarrow>
    reduceContractStep env state (Pay accId payee val cont) = Reduced wa eff newState newCont \<Longrightarrow>
-   0 \<le> moneyInAccount y (accounts newState)"
+   positiveMoneyInAccountOrNoAccount y (accounts newState)"
   apply (simp only:reduceContractStep.simps)
   apply (cases "evalValue env state val \<le> 0")
   apply simp
   apply (cases "giveMoney payee (min (moneyInAccount accId (accounts state)) (evalValue env state val))
                 (updateMoneyInAccount accId (moneyInAccount accId (accounts state) - min (moneyInAccount accId (accounts state)) (evalValue env state val))
                   (accounts state))")
-  apply (simp del:moneyInAccount.simps valid_state.simps updateMoneyInAccount.simps)
-  by (smt MList_delete_preserves_geZero ReduceStepResult.inject State.select_convs(1) State.surjective State.update_convs(1) giveMoney_geZero updateMoneyInAccount.simps updateMoneyInAccount_geZero valid_state.elims(2))
+  apply (simp del:positiveMoneyInAccountOrNoAccount.simps valid_state.simps updateMoneyInAccount.simps)
+  by (smt MList_delete_preserves_gtZero ReduceStepResult.inject State.select_convs(1) State.surjective State.update_convs(1) giveMoney_gtZero updateMoneyInAccount.simps updateMoneyInAccount_gtZero valid_state.elims(2))
 
-lemma reduceContractStep_geZero_Let :
+lemma reduceContractStep_gtZero_Let :
   "valid_state state \<Longrightarrow>
-   \<forall>x. 0 \<le> moneyInAccount x (accounts state) \<Longrightarrow>
+   \<forall>x. positiveMoneyInAccountOrNoAccount x (accounts state) \<Longrightarrow>
    reduceContractStep env state (Contract.Let valueId val cont) = Reduced wa eff newState newCont \<Longrightarrow>
-   0 \<le> moneyInAccount y (accounts newState)"
+   positiveMoneyInAccountOrNoAccount y (accounts newState)"
   apply (simp only:reduceContractStep.simps)
   apply (cases "state")
   apply (cases "newState")
-  apply (simp del:moneyInAccount.simps valid_state.simps)
+  apply (simp del:positiveMoneyInAccountOrNoAccount.simps valid_state.simps)
   by (metis ReduceStepResult.inject State.ext_inject)
 
-theorem reduceContractStep_geZero :
+theorem reduceContractStep_gtZero :
   "valid_state state \<Longrightarrow>
-   (\<forall>x. moneyInAccount x (accounts state) \<ge> 0) \<Longrightarrow>
+   (\<forall>x. positiveMoneyInAccountOrNoAccount x (accounts state)) \<Longrightarrow>
    reduceContractStep env state cont = Reduced wa eff newState newCont \<Longrightarrow>
-   moneyInAccount y (accounts newState) \<ge> 0"
+   positiveMoneyInAccountOrNoAccount y (accounts newState)"
   apply (cases cont)
   apply (cases "refundOne (accounts state)")
   apply simp
-  using reduceContractStep_geZero_Refund apply force
-  using reduceContractStep_geZero_Pay apply blast
+  using reduceContractStep_gtZero_Refund apply force
+  using reduceContractStep_gtZero_Pay apply blast
   apply simp
   apply (smt ReduceStepResult.distinct(1) ReduceStepResult.inject ReduceStepResult.simps(5) case_prod_unfold reduceContractStep.simps(4))
-  using reduceContractStep_geZero_Let by blast
+  using reduceContractStep_gtZero_Let by blast
 
 (* Alternative formulation *)
 
@@ -161,19 +168,18 @@ fun allAccountsPositive :: "(AccountId \<times> Money) list \<Rightarrow> bool" 
 fun allAccountsPositiveState :: "State \<Rightarrow> bool" where
 "allAccountsPositiveState state = allAccountsPositive (accounts state)"
 
-lemma positiveMoneyInAccount :
-  "allAccountsPositive accs \<Longrightarrow> 0 < moneyInAccount accId accs"
+lemma allAccountsPositiveImpliesPositiveMoneyInAccountOrNoAccount :
+  "allAccountsPositive accs \<Longrightarrow> positiveMoneyInAccountOrNoAccount accId accs"
   oops
 
-lemma addMoneyToAccountPositive :
-  "0 \<le> money \<and> allAccountsPositive accs
-  \<Longrightarrow> allAccountsPositive (addMoneyToAccount accId money accs)"
+lemma positiveMoneyInAccountOrNoAccountImpliesAllAccountsPositive :
+  "(\<forall> accId. positiveMoneyInAccountOrNoAccount accId accs) \<Longrightarrow> allAccountsPositive accs"
   oops
 
 theorem accountsArePositive :
-"(\<forall>x. moneyInAccount x (accounts state) \<ge> 0) \<Longrightarrow>
+"(\<forall>x. positiveMoneyInAccountOrNoAccount x (accounts state)) \<Longrightarrow>
   computeTransaction txIn state cont = TransactionOutput txOut \<Longrightarrow>
-  moneyInAccount y (accounts (txOutState txOut)) \<ge> 0"
+  positiveMoneyInAccountOrNoAccount y (accounts (txOutState txOut))"
 oops
 
 theorem accountsArePositive2 :
